Hybrid/Proof/Lemmas.lean
@@ -286,10 +286,10 @@ end PremiseLemmas
 
 section Lindenbaum
 
-  lemma name' {i : symbs.nominal s} (h1 : ¬Λ.occurs i ) (h2 : φ.occurs i = false) : ⊢(Λ, s) (i ⟶ φ) → ⊢(Λ, s) φ := by
+  lemma name' {i : symbs.nomType s} (h2 : φ.occurs i = false) : ⊢(Λ, s) (i ⟶ φ) → ⊢(Λ, s) φ := by
     intro (.intro pf)
     apply Nonempty.intro
-    exact name'_proof h1 h2 pf
+    exact name'_proof h2 pf
 
   lemma q2_nom' (h1 : ¬Λ.occurs i) (h2 : φ.occurs i = false) : ⊢(Λ, s) (ℋ@ i (ℋVar x) ⟶ φ) → ⊢(Λ, s) φ := by
     intro (.intro pf)
@@ -322,7 +322,7 @@ section Lindenbaum
 
   lemma paste_consistent {s} {Λ : AxiomSet symbs} {Γ : PremiseSet symbs s}
     (h1 : Γ.consistent Λ) (h2 : ℋ@ j (ℋ⟨σ⟩ φ) ∈ Γ) {e : φ.Elem}
-    {i : symbs.nominal e.1} (h3 : ¬Λ.occurs i) (h4 : ¬Γ.occurs i):
+    {i : symbs.nomType e.1} (h4 : ¬Γ.occurs i):
     (Γ ∪ {ℋ@ j (ℋ⟨σ⟩ e.2.2[ℋNom i]) ⋀ ℋ@ i e.2.1}).consistent Λ := by
       rename_i t _ _
       intro habs
@@ -334,7 +334,7 @@ section Lindenbaum
         let C := (ℋNom i).subst_to_ctx e.2.2
         /- Proving restrictions for Paste rule -/
         have subst_is_φ : C[e.2.1] = φ := e.2.2.subst_in_iso $ (ℋNom i).subst_to_ctx_iso e.2.2
-        have neq_nom : i ≠ₛ j := by
+        have neq_nom : .nom i ≠ₛ j := by
           intro heq
           by_cases trivial : e.1 = t
           . subst trivial
@@ -345,7 +345,7 @@ section Lindenbaum
             apply And.intro h2
             simp [FormL.occurs, Term.occurs, FormL.nom_occurs]
           . contradiction
-        have nocc_conj : (Γ_list.conjunction ⟶ ℋ⊥).occurs i = false := by
+        have nocc_conj : (Γ_list.conjunction ⟶ ℋ⊥).occurs (.nom i : symbs.nominal e.1) = false := by
           simp only [FormL.occurs_nom_implies, FormL.occurs_nom_bot, Bool.or_false]
           apply nominal_not_occurs_premise h4
         have nocc_φ : C[e.2.1].occurs i = false := by
@@ -355,7 +355,7 @@ section Lindenbaum
           simp only [FormL.occurs, Term.occurs, FormL.nom_occurs, Bool.or_eq_false_iff] at h4
           exact h4.1
         /- Done, now applying Paste rule  -/
-        have l2 := subst_is_φ ▸ paste C neq_nom h3 nocc_conj nocc_φ l1
+        have l2 := subst_is_φ ▸ paste C neq_nom nocc_conj nocc_φ l1
         have l3 : Γ ⊢(Λ) (_ ⟶ ℋ⊥) := ⟨Γ_list, ⟨imp_com_proof l2⟩⟩
         have l4 : Γ ⊢(Λ) _ := premise_provable h2
         have l4 := premise_mp l3 l4
